Tested Nominal CompCert with Structured Memory Space

driver/Interp.ml
@@ -128,7 +128,7 @@ let print_state p (prog, ge, s) =
       fprintf p "in function %s, expression@ @[<hv 0>%a@]"
               (name_of_function prog f)
               PrintCsyntax.print_expr r
-  | Callstate(fd, args, k, m) ->
+  | Callstate(fd, args, k, m, id) ->
       PrintCsyntax.print_pointer_hook := print_pointer ge.genv_genv Maps.PTree.empty;
       fprintf p "calling@ @[<hov 2>%s(%a)@]"
               (name_of_fundef prog fd)
@@ -234,14 +234,16 @@ let rank_state = function
 let mem_state = function
   | State(f, s, k, e, m) -> m
   | ExprState(f, r, k, e, m) -> m
-  | Callstate(fd, args, k, m) -> m
+  | Callstate(fd, args, k, m, id) -> m
   | Returnstate(res, k, m) -> m
   | Stuckstate -> assert false
 
 let compare_state s1 s2 =
   if s1 == s2 then 0 else
-  let c = compare_sup (mem_state s1).Mem.support (mem_state s2).Mem.support in
-  if c <> 0 then c else begin
+  let c = compare_sup (mem_state s1).Mem.support.Mem.global
+      (mem_state s2).Mem.support.Mem.global in
+  if c <> 0 then c else
+  begin
   match s1, s2 with
   | State(f1,s1,k1,e1,m1), State(f2,s2,k2,e2,m2) ->
       let c = compare (f1,s1,e1) (f2,s2,e2) in if c <> 0 then c else
@@ -251,7 +253,8 @@ let compare_state s1 s2 =
       let c = compare (f1,r1,e1) (f2,r2,e2) in if c <> 0 then c else
       let c = compare_cont k1 k2 in if c <> 0 then c else
       compare_mem m1 m2
-  | Callstate(fd1,args1,k1,m1), Callstate(fd2,args2,k2,m2) ->
+  | Callstate(fd1,args1,k1,m1,id1), Callstate(fd2,args2,k2,m2,id2) ->
+      let c = compare id1 id2 in if c <> 0 then c else
       let c = compare (fd1,args1) (fd2,args2) in if c <> 0 then c else
       let c = compare_cont k1 k2 in if c <> 0 then c else
       compare_mem m1 m2
@@ -327,8 +330,8 @@ let format_value m flags length conv arg =
       end
   | 's', "", _ ->
       "<pointer argument expected>"
-  | 'p', "", Vptr(blk, ofs) ->
-      Printf.sprintf "<%ld%+ld>" (P.to_int32 blk) (camlint_of_coqint ofs)
+  | 'p', "", Vptr(Global id, ofs) ->
+      Printf.sprintf "<%ld%+ld>" (P.to_int32 id) (camlint_of_coqint ofs)
   | 'p', "", Vint i ->
       format_int32 (flags ^ "x") (camlint_of_coqint i)
   | 'p', "", _ ->
